Refinement

Export.thy
@@ -4,34 +4,34 @@ begin
 
 datatype TypeToken = LParen | RParen | LBrack | RBrack | Comma | Elem string
 
-primrec explode1 :: "string \<Rightarrow> TypeToken list" where
-  "explode1 (x#tail) = Elem [x]#explode1 tail"
-| "explode1 [] = []"
+primrec typeTokenExplode :: "string \<Rightarrow> TypeToken list" where
+  "typeTokenExplode (x#tail) = Elem [x]#typeTokenExplode tail"
+| "typeTokenExplode [] = []"
 
-fun scanParens :: "TypeToken list \<Rightarrow> TypeToken list" where
-  "scanParens (Elem ''(''#tail) = LParen#scanParens tail"
-| "scanParens (Elem '')''#tail) = RParen#scanParens tail"
-| "scanParens (z#tail) = z#scanParens tail"
-| "scanParens [] = []"
+fun typeTokenScanParens :: "TypeToken list \<Rightarrow> TypeToken list" where
+  "typeTokenScanParens (Elem ''(''#tail) = LParen#typeTokenScanParens tail"
+| "typeTokenScanParens (Elem '')''#tail) = RParen#typeTokenScanParens tail"
+| "typeTokenScanParens (z#tail) = z#typeTokenScanParens tail"
+| "typeTokenScanParens [] = []"
 
-fun scanBrackets :: "TypeToken list \<Rightarrow> TypeToken list" where
-  "scanBrackets (Elem ''[''#tail) = LBrack#scanBrackets tail"
-| "scanBrackets (Elem '']''#tail) = RBrack#scanBrackets tail"
-| "scanBrackets (z#tail) = z#scanBrackets tail"
-| "scanBrackets [] = []"
+fun typeTokenScanBrackets :: "TypeToken list \<Rightarrow> TypeToken list" where
+  "typeTokenScanBrackets (Elem ''[''#tail) = LBrack#typeTokenScanBrackets tail"
+| "typeTokenScanBrackets (Elem '']''#tail) = RBrack#typeTokenScanBrackets tail"
+| "typeTokenScanBrackets (z#tail) = z#typeTokenScanBrackets tail"
+| "typeTokenScanBrackets [] = []"
 
-fun scanComma :: "TypeToken list \<Rightarrow> TypeToken list" where
-  "scanComma (Elem '',''#tail) = Comma#scanComma tail"
-| "scanComma (z#tail) = z#scanComma tail"
-| "scanComma [] = []"
+fun typeTokenScanCommas :: "TypeToken list \<Rightarrow> TypeToken list" where
+  "typeTokenScanCommas (Elem '',''#tail) = Comma#typeTokenScanCommas tail"
+| "typeTokenScanCommas (z#tail) = z#typeTokenScanCommas tail"
+| "typeTokenScanCommas [] = []"
 
-fun scanCombine :: "TypeToken list \<Rightarrow> TypeToken list" where
-  "scanCombine (Elem a#Elem b#tail) = scanCombine (Elem (a@b)#tail)"
-| "scanCombine (y#tail) = y#scanCombine tail"
-| "scanCombine [] = []"
+fun typeTokenCombine :: "TypeToken list \<Rightarrow> TypeToken list" where
+  "typeTokenCombine (Elem a#Elem b#tail) = typeTokenCombine (Elem (a@b)#tail)"
+| "typeTokenCombine (y#tail) = y#typeTokenCombine tail"
+| "typeTokenCombine [] = []"
 
-definition scan :: "string \<Rightarrow> TypeToken list" where
-  "scan \<equiv> \<lambda> input. scanCombine (scanComma (scanBrackets (scanParens (explode1 input))))"
+definition scanTypeTokens :: "string \<Rightarrow> TypeToken list" where
+  "scanTypeTokens \<equiv> typeTokenCombine o typeTokenScanCommas o typeTokenScanBrackets o typeTokenScanParens o typeTokenExplode"
 
 definition is_digit :: "char \<Rightarrow> bool" where
   "is_digit \<equiv> \<lambda> c . ((of_char c)::nat) \<ge> ((of_char (CHR ''0''))) \<and> ((of_char c)::nat) \<le> ((of_char (CHR ''9'')))"
@@ -52,10 +52,6 @@ fun splitDigitSuffix :: "string \<Rightarrow> string \<Rightarrow> (string \<tim
       splitDigitSuffix tail (x#parsed))"
 | "splitDigitSuffix [] parsed = (List.rev parsed,None)"
 
-
-
-term "x::char"
-
 definition ParseBaseTypePrefix :: "string \<Rightarrow> (nat option \<Rightarrow> abi_type option) option" where
   "ParseBaseTypePrefix \<equiv> [
     ''uint'' \<mapsto> (\<lambda> nopt . map_option (\<lambda> n . Tuint n) nopt),
@@ -65,75 +61,123 @@ definition ParseBaseTypePrefix :: "string \<Rightarrow> (nat option \<Rightarrow
     ''bool'' \<mapsto> (\<lambda> opt . case opt of None \<Rightarrow> Some Tbool | _ \<Rightarrow> None),
     ''bytes'' \<mapsto> (\<lambda> opt . case opt of Some n \<Rightarrow> Some (Tfbytes n) | _ \<Rightarrow> Some Tbytes),
     ''string'' \<mapsto> (\<lambda> opt . case opt of None \<Rightarrow> Some (Tstring) | _ \<Rightarrow> None)
-]"
+  ]"
 
 definition ParseBaseType :: "string \<Rightarrow> abi_type option" where
   "ParseBaseType \<equiv> \<lambda> str . case (splitDigitSuffix str []) of (prefix, nopt) \<Rightarrow>
-  (case ParseBaseTypePrefix prefix of Some fn \<Rightarrow> fn nopt | _ \<Rightarrow> None)
-"
+    (case ParseBaseTypePrefix prefix of Some fn \<Rightarrow> fn nopt | _ \<Rightarrow> None)"
 
-datatype Type = Type abi_type | Tuple "Type list" | Array Type string
+datatype typeParserState = tPS_primary abi_type | tPS_array abi_type "nat option" | tPS_tuple "abi_type list"
 
-fun TypeM :: "Type \<Rightarrow> nat" where
-  "TypeM (Type _) = 1"
-| "TypeM (Tuple x) = length x + sum_list (map TypeM x)"
-| "TypeM (Array x []) = 2 + TypeM x"
-| "TypeM (Array x y) = 3 + TypeM x"
+fun typeParser :: "TypeToken list \<Rightarrow> typeParserState list \<Rightarrow> abi_type option" where
+  "typeParser (LParen#tail) st = typeParser tail (tPS_tuple []#st)"
+| "typeParser (Elem x#tail) (tPS_array t None#st) = Option.bind (parseNat x) (\<lambda> n . typeParser tail (tPS_array t (Some n)#st))"
+| "typeParser (Elem x#tail) [] = Option.bind (ParseBaseType x) (\<lambda> type . typeParser tail (tPS_primary type#[]))"
+| "typeParser (Elem x#tail) (tPS_tuple t#ts) = Option.bind (ParseBaseType x) (\<lambda> type . typeParser tail (tPS_primary type#tPS_tuple t#ts))"
+| "typeParser (LBrack#tail) (tPS_primary x#st) = typeParser tail (tPS_array x None#st)"
+| "typeParser (RBrack#tail) (tPS_array x nopt#st) = typeParser tail (tPS_primary (case nopt of Some n \<Rightarrow> Tfarray x n | _ \<Rightarrow> Tarray x)#st)"
+| "typeParser (RParen#tail) (tPS_primary t#tPS_tuple ts#st) = typeParser tail (tPS_primary (Ttuple (List.rev (t#ts)))#st)"
+| "typeParser (Comma#tail) (tPS_primary t#tPS_tuple ts#st) = typeParser tail (tPS_tuple (t#ts)#st)"
+| "typeParser [] [tPS_primary x] = Some x"
+| "typeParser _ _ = None"
 
-fun M :: "TypeToken list + TypeToken list + (TypeToken list \<times> Type list) \<Rightarrow> nat" where
-  "M (Inl x) = length x"
-| "M (Inr (Inl x)) = length x"
-| "M (Inr (Inr (x, y))) = 1 + length x + sum_list (map TypeM y)"
+definition parseType :: "string \<Rightarrow> abi_type option" where
+  "parseType \<equiv> \<lambda> x . typeParser (scanTypeTokens x) []"
 
-term "char_of"
-term "of_char"
+value "parseType ''(uint256[2][1],(uint8,uint9),uint256)''"
 
-function (sequential) parse :: "TypeToken list \<Rightarrow> (TypeToken list \<times> abi_type) option" and
-    parseArray :: "TypeToken list \<Rightarrow> (TypeToken list \<times> abi_type) option" and 
-    parseTuple :: "TypeToken list \<Rightarrow> abi_type list \<Rightarrow> (TypeToken list \<times> abi_type list) option" where
-  "parse (RBrack#tail) = parseArray tail"
-| "parse (Elem x#tail) = (case ParseBaseType x of Some type \<Rightarrow> Some (tail, type) | _ \<Rightarrow> None)"
-| "parse (RParen#tail) = (case parseTuple tail [] of Some (tail, types) \<Rightarrow> Some (tail, Ttuple (List.rev types)) | _ \<Rightarrow> None)"
-| "parse _ = None"
-| "parseArray (LBrack#tail) = (case parse tail of Some (tail, type) \<Rightarrow> Some (tail,Tarray type) | _ \<Rightarrow> None)"
-| "parseArray (Elem x#LBrack#tail) = (case parse tail of Some (tail, type) \<Rightarrow>
-    (case parseNat x of (Some n) \<Rightarrow> Some (tail, Tfarray type n) | _ \<Rightarrow> None)
-     | _ \<Rightarrow> None
-)"
-| "parseArray oth = None"
-| "parseTuple (LParen#tail) staged = Some (tail, staged)"
-| "parseTuple [] staged = None"
-| "parseTuple oth staged = (case parse oth of Some (LParen#tail, type) \<Rightarrow> Some (tail, type#staged)
-                                              | Some (Comma#tail, type) \<Rightarrow> (
-            case (parseTuple tail []) of Some (tail, types) \<Rightarrow> Some (tail, type#types) | _ \<Rightarrow> None
-)
-                                              | _ \<Rightarrow> None)"
-  by auto pat_completeness
+definition parseHexDigit :: "char \<Rightarrow> int option" where
+  "parseHexDigit x \<equiv> 
+    if is_digit x
+    then Some (((of_char x)::int) - of_char (CHR ''0''))
+    else if (((of_char x)::nat) \<ge> of_char (CHR ''A'') \<and> ((of_char x)::nat) \<le> of_char (CHR ''F''))
+    then Some (((of_char x)::int) - of_char (CHR ''A'') + 10)
+    else if (((of_char x)::nat) \<ge> of_char (CHR ''a'') \<and> ((of_char x)::nat) \<le> of_char (CHR ''f''))
+    then Some (((of_char x)::int) - of_char (CHR ''a'') + 10)
+    else None"
 
-termination 
-  sorry (* TODO *)
+definition parseWord :: "char \<Rightarrow> char \<Rightarrow> 8 word option" where
+  "parseWord \<equiv> \<lambda> x y . case (parseHexDigit x, parseHexDigit y) of (Some x, Some y) \<Rightarrow> Some (word_of_int (x * 16 + y)) | _ \<Rightarrow> None"
 
-definition readType :: "string \<Rightarrow> abi_type option" where
-  "readType \<equiv> \<lambda> x . case (parse (List.rev (scan x))) of Some ([], x) \<Rightarrow> Some x | _ \<Rightarrow> None"
+fun parseWords :: "string \<Rightarrow> 8 word list option" where
+  "parseWords (x#y#z) = (case (parseWord x y, parseWords z) of (Some b, Some bs) \<Rightarrow> Some (b#bs) | _ \<Rightarrow> None)"
+| "parseWords [] = Some []"
+| "parseWords [x] = None"
 
-value "parse (List.rev (scan ''(uint256[2][1])''))"
-value "readType ''(uint256[2][1],(uint8,uint9),uint256)''"
+datatype valueParseTree = arrayValue "valueParseTree list" | tupleValue "valueParseTree list" | primaryValue string
+datatype valueParserState = vPS_primary valueParseTree | vPS_arrtuple bool "valueParseTree list"
+fun valueParser :: "TypeToken list \<Rightarrow> valueParserState list \<Rightarrow> valueParseTree option" where
+  "valueParser (Elem x#[]) [] = Some (primaryValue x)"
+| "valueParser (Elem x#tail) (vPS_arrtuple w ar#st) = valueParser tail ((vPS_primary (primaryValue x))#vPS_arrtuple w ar#st)"
+| "valueParser (LBrack#tail) (st) = valueParser tail (vPS_arrtuple False []#st)"
+| "valueParser (LParen#tail) (st) = valueParser tail (vPS_arrtuple True []#st)"
+| "valueParser (RBrack#tail) (vPS_arrtuple False arr#st) = valueParser tail ((vPS_primary (arrayValue []))#st)"
+| "valueParser (RBrack#tail) (vPS_primary x#vPS_arrtuple False arr#st) = valueParser tail ((vPS_primary (arrayValue (List.rev (x#arr))))#st)"
+| "valueParser (RParen#tail) (vPS_primary x#vPS_arrtuple True arr#st) = valueParser tail ((vPS_primary (tupleValue (List.rev (x#arr))))#st)"
+| "valueParser (Comma#tail) (vPS_primary x#vPS_arrtuple w arr#st) = valueParser tail (vPS_arrtuple w (x#arr)#st)"
+| "valueParser [] [vPS_primary y] = Some y"
+| "valueParser _ _ = None"
+
+definition parseU256 :: "string \<Rightarrow> 256 word option" where
+  "parseU256 \<equiv> \<lambda> str. (case parseWords str of Some w \<Rightarrow> (if length w = 32 then Some (word_rcat w) else None) | _ \<Rightarrow> None)"
+
+function (sequential) typedValueParser :: "abi_type \<Rightarrow> valueParseTree \<Rightarrow> abi_value option" where
+  "typedValueParser (Tuint n) (primaryValue v) = map_option (\<lambda> w . Vuint n (uint w)) (parseU256 v)"
+| "typedValueParser (Tsint n) (primaryValue v) = map_option (\<lambda> w . Vsint n (sint w)) (parseU256 v)"
+| "typedValueParser Taddr (primaryValue v) = map_option (\<lambda> w . Vaddr (uint w)) (parseU256 v)"
+| "typedValueParser (Tfarray t n) (arrayValue vs) = (if (length vs = n) then map_option (\<lambda> vs . Vfarray t n vs) (those (map (\<lambda> v . typedValueParser t v) vs))  else None)"
+| "typedValueParser (Tarray t) (arrayValue vs) = (map_option (\<lambda> vs . Varray t vs) (those (map (\<lambda> v . typedValueParser t v) vs)))"
+| "typedValueParser (Ttuple ts) (tupleValue vs) = (if (length vs = length ts) then map_option (\<lambda> vs . Vtuple ts vs) (those (map2 (\<lambda> t v . typedValueParser t v) ts vs)) else None)"
+| "typedValueParser _ _ = None"
+  by pat_completeness auto
+
+primrec valueParseTreeMeasure :: "valueParseTree \<Rightarrow> nat" where
+  "valueParseTreeMeasure (primaryValue x) = 1"
+| "valueParseTreeMeasure (arrayValue xs) = 1 + (List.foldl (+) 0 (map valueParseTreeMeasure xs))"
+| "valueParseTreeMeasure (tupleValue xs) = 1 + (List.foldl (+) 0 (map valueParseTreeMeasure xs))"
+
+termination proof -
+  have "x \<in> set vs \<Longrightarrow> valueParseTreeMeasure x \<in> set (map valueParseTreeMeasure vs)" for x vs by auto
+  moreover have "(x::nat) \<in> set y \<Longrightarrow> List.foldl (+) 0 y \<ge> x" for x y
+  proof -
+    have 0: "foldl (+) (x + a) yb = a + foldl (+) x yb" for x a ::nat and yb
+      by (induct yb arbitrary: a) (auto simp: add.assoc)
+    assume "(x::nat) \<in> set y"
+    then obtain ya yb where y_def: "y = ya@[x]@yb"
+      by (metis append_Cons append_Nil split_list)
+    show "List.foldl (+) 0 y \<ge> x" unfolding y_def
+      using 0 by simp
+  qed
+  ultimately show ?thesis 
+    by (relation "measure (\<lambda>(x,y) . valueParseTreeMeasure y)")
+       (auto simp: less_SucI set_zip_rightD le_imp_less_Suc)
+qed
+
+value "Option.bind (parseType ''int256[]'') (\<lambda> t . Option.bind (valueParser (scanTypeTokens ''[0000000000000000000000000000000000000000000000000000000000000010,0000000000000000000000000000000000000000000000000000000000000011]'') []) (\<lambda> v . typedValueParser t v))"
+
+definition parseTypedValue :: "abi_type \<Rightarrow> string \<Rightarrow> abi_value option" where
+  "parseTypedValue \<equiv> \<lambda>type str . Option.bind (valueParser (scanTypeTokens str) []) (\<lambda> vs . typedValueParser type vs)"
+
+value "Option.bind (parseType ''int256[0]'') (\<lambda> t. parseTypedValue t ''[]'')"
+
 (*
-fun writeNat :: "nat \<Rightarrow> string" where
-  "writeNat x = (if x < 10 then [char_of (of_char (CHR ''0'') + x)] else writeNat (x div 10)@writeNat (x mod 10))"
-
-
-definition writeInt :: "int \<Rightarrow> string" where
-  "writeInt \<equiv> (\<lambda> x . if x < 0 then CHR ''-''#writeNat (nat (-x)) else writeNat (nat x))"
+  "valueParser (LParen#tail) st = valueParser tail (tupleValue []#st)"
+| "valueParser (Elem x#[]) [] = Some (primaryValue x)"
+| "valueParser (Elem x#tail) (arrayValue vs#st) = valueParser"
+| "valueParser (Elem x#tail) (tPS_tuple t#ts) = Option.bind (ParseBaseType x) (\<lambda> type . typeParser tail (tPS_primary type#tPS_tuple t#ts))"
+| "valueParser (LBrack#tail) (tPS_primary x#st) = typeParser tail (tPS_array x None#st)"
+| "valueParser (RBrack#tail) (tPS_array x nopt#st) = typeParser tail (tPS_primary (case nopt of Some n \<Rightarrow> Tfarray x n | _ \<Rightarrow> Tarray x)#st)"
+| "valueParser (RParen#tail) (tPS_primary t#tPS_tuple ts#st) = typeParser tail (tPS_primary (Ttuple (List.rev (t#ts)))#st)"
+| "valueParser (Comma#tail) (tPS_primary t#tPS_tuple ts#st) = typeParser tail (tPS_tuple (t#ts)#st)"
+| "valueParser [] [tPS_primary x] = Some x"
+| "valueParser _ _ = None"
 *)
-
 
 fun writeHexNibble :: "4 word \<Rightarrow> char" where
   "writeHexNibble x = (if x < 10 then char_of (of_char (CHR ''0'') + uint x) else char_of (of_char (CHR ''A'') + uint x - 10))"
 
 fun writeHexDigit :: "8 word \<Rightarrow> string" where
   "writeHexDigit x = (writeHexNibble (ucast (x >> 4)))#[writeHexNibble (ucast (x AND 0xF))]"
-
 
 fun writeHex :: "8 word list \<Rightarrow> string" where
   "writeHex (x#tail) = writeHexDigit x@writeHex tail"
@@ -160,7 +204,6 @@ primrec writeType :: "abi_type \<Rightarrow> string" and
 | "writeTypeList (t#ts) = (if ts = [] then writeType t else writeType t@'',''@writeTypeList ts)"
 | "writeTypeList [] = ''''"
 
-
 primrec writeValue :: "abi_value \<Rightarrow> string" and writeValueList :: "abi_value list \<Rightarrow> string" where
   "writeValue (Vuint s value) = writeInt value"
 | "writeValue (Vsint s value) = writeInt value"
@@ -178,44 +221,19 @@ primrec writeValue :: "abi_value \<Rightarrow> string" and writeValueList :: "ab
 | "writeValue (Vbytes v) = ''0x''@(writeHex v)"
 | "writeValue (Vstring str) = ''0x''@writeHex (map (\<lambda> x . word_of_int (of_char x)) str)"
 
-term "decode"
-
-definition parseHexDigit :: "char \<Rightarrow> int option" where
-  "parseHexDigit x \<equiv> (if (((of_char x)::nat) \<ge> of_char (CHR ''0'') \<and> ((of_char x)::nat) \<le> of_char (CHR ''9'')) then
-                        Some (((of_char x)::int) - of_char (CHR ''0''))
-                      else (
-  if (((of_char x)::nat) \<ge> of_char (CHR ''A'') \<and> ((of_char x)::nat) \<le> of_char (CHR ''F'')) then
-                        Some (((of_char x)::int) - of_char (CHR ''A'') + 10)
-  else (  if (((of_char x)::nat) \<ge> of_char (CHR ''a'') \<and> ((of_char x)::nat) \<le> of_char (CHR ''f'')) then
-                        Some (((of_char x)::int) - of_char (CHR ''a'') + 10)
-  else
-None
-)
-) )"
-
-
-definition parseWord :: "char \<Rightarrow> char \<Rightarrow> 8 word option" where
-  "parseWord \<equiv> \<lambda> x y . case (parseHexDigit x, parseHexDigit y) of (Some x, Some y) \<Rightarrow> Some (word_of_int (x * 16 + y)) | _ \<Rightarrow> None"
-
-fun parseWords :: "string \<Rightarrow> 8 word list option" where
-  "parseWords (x#y#z) = (case (parseWord x y, parseWords z) of (Some b, Some bs) \<Rightarrow> Some (b#bs) | _ \<Rightarrow> None)"
-| "parseWords [] = Some []"
-| "parseWords [x] = None"
-
-term "case_option"
-
 definition Decode :: "String.literal \<Rightarrow> String.literal \<Rightarrow> String.literal" where
-  "Decode \<equiv> \<lambda> type encoding . 
-    case (Option.bind (readType (literal.explode type))
-      (\<lambda> type . map_option (\<lambda> encoding . decode type encoding) (parseWords (literal.explode encoding))))
-      of (Some result) \<Rightarrow> (case result of (Ok value) \<Rightarrow> String.implode (writeValue value) | (Err reason) \<Rightarrow> String.implode (''ERR: ''@reason)
-) | _ \<Rightarrow> String.implode ''ERR: INVALID INPUT''"
-
-value "decode (Ttuple [Tuint 256,Tuint 256]) (the (parseWords ''000102030405060708090A0B0C0D0E0F101112131415161718191A1B1C1D1E1F000000000000000000000000000000000000000000000000000000000000001F''))"
-
-value "readType ''(uint248,uint8)''"
-
-value "Decode (String.implode ''(uint248,uint8[1])'') (String.implode ''000102030405060708090A0B0C0D0E0F101112131415161718191A1B1C1D1E1F000000000000000000000000000000000000000000000000000000000000001F'')"
+  "Decode \<equiv> \<lambda> type encoding .
+    case parseType (literal.explode type) of Some type \<Rightarrow>
+    (
+      case parseWords (literal.explode encoding) of Some encoding \<Rightarrow>
+      (
+        case decode type encoding of (Ok value) \<Rightarrow> String.implode (''OK: ''@writeValue value)
+        | Err msg \<Rightarrow> String.implode (''ERR: ''@msg)
+      )
+      | _ \<Rightarrow> String.implode ''ERR: Cannot parse encoding.''
+    )
+    | _ \<Rightarrow> String.implode ''ERR: Cannot parse type.''
+"
 
 export_code Decode in SML module_name ABICoder file_prefix abicoder
 
